Change `Imperative.Stmt` to remove `Block` mutual recursion (#216)
Makes some definitions cleaner as they no longer need angle brackets or
`{ss := _}`.

`Block` is now an `abbrev` for `List Stmt`, and we don't need both
`Stmts` and `Block`. This makes the semantics for statements cleaner.

This also includes an induction principle for the new version of `Stmt`,
though it is unused right now.


By submitting this pull request, I confirm that you can use, modify,
copy, and redistribute this contribution, under the terms of your
choice.

---------

Co-authored-by: Josh Cohen <cohenjo@amazon.com>
Co-authored-by: Andrew Wells <130512013+andrewmwells-amazon@users.noreply.github.com>
Co-authored-by: Andrew Wells <anmwells@amazon.com>

Strata/DL/Imperative/Stmt.lean
@@ -17,28 +17,59 @@ Imperative's Statements include commands and add constructs like structured and
 unstructured control-flow.
 -/
 
-mutual
 inductive Stmt (P : PureExpr) (Cmd : Type) : Type where
   | cmd      (cmd : Cmd)
-  | block    (label : String) (b : Block P Cmd) (md : MetaData P := .empty)
+  | block    (label : String) (b : List (Stmt P Cmd)) (md : MetaData P := .empty)
   /-- `ite` (if-then-else) statement provides structured control flow. -/
-  | ite      (cond : P.Expr)  (thenb : Block P Cmd) (elseb : Block P Cmd) (md : MetaData P := .empty)
+  | ite      (cond : P.Expr)  (thenb : List (Stmt P Cmd)) (elseb : List (Stmt P Cmd)) (md : MetaData P := .empty)
   /-- `loop` Loop statement with optional measure (for termination) and invariant. -/
-  | loop     (guard : P.Expr) (measure : Option P.Expr) (invariant : Option P.Expr) (body : Block P Cmd) (md : MetaData P := .empty)
+  | loop     (guard : P.Expr) (measure : Option P.Expr) (invariant : Option P.Expr) (body : List (Stmt P Cmd)) (md : MetaData P := .empty)
   /-- `goto` provides unstructured control flow. -/
   | goto     (label : String) (md : MetaData P := .empty)
   deriving Inhabited
 
-structure Block (P : PureExpr) (Cmd : Type) where
-  ss : List (Stmt P Cmd)
-end
-
-abbrev Stmts (P : PureExpr) (Cmd : Type) := List (Stmt P Cmd)
+abbrev Block (P : PureExpr) (Cmd : Type) := List (Stmt P Cmd)
 
 def Stmt.isCmd {P : PureExpr} {Cmd : Type} (s : Stmt P Cmd) : Bool :=
   match s with
   | .cmd _ => true
   | _ => false
+
+
+/--
+Induction principle for `Stmt`
+-/
+@[elab_as_elim]
+def Stmt.inductionOn {P : PureExpr} {Cmd : Type}
+    {motive : Stmt P Cmd → Sort u}
+    (cmd_case : ∀ (cmd : Cmd), motive (Stmt.cmd cmd))
+    (block_case : ∀ (label : String) (b : List (Stmt P Cmd)) (md : MetaData P),
+      (∀ s, s ∈ b → motive s) →
+      motive (Stmt.block label b md))
+    (ite_case : ∀ (cond : P.Expr) (thenb elseb : List (Stmt P Cmd)) (md : MetaData P),
+      (∀ s, s ∈ thenb → motive s) →
+      (∀ s, s ∈ elseb → motive s) →
+      motive (Stmt.ite cond thenb elseb md))
+    (loop_case : ∀ (guard : P.Expr) (measure invariant : Option P.Expr)
+      (body : List (Stmt P Cmd)) (md : MetaData P),
+      (∀ s, s ∈ body → motive s) →
+      motive (Stmt.loop guard measure invariant body md))
+    (goto_case : ∀ (label : String) (md : MetaData P),
+      motive (Stmt.goto label md))
+    (s : Stmt P Cmd) : motive s :=
+  match s with
+  | Stmt.cmd c => cmd_case c
+  | Stmt.block label b md =>
+    block_case label b md (fun s _ => inductionOn cmd_case block_case ite_case loop_case goto_case s)
+  | Stmt.ite cond thenb elseb md =>
+    ite_case cond thenb elseb md
+      (fun s _ => inductionOn cmd_case block_case ite_case loop_case goto_case s)
+      (fun s _ => inductionOn cmd_case block_case ite_case loop_case goto_case s)
+  | Stmt.loop guard measure invariant body md =>
+    loop_case guard measure invariant body md
+      (fun s _ => inductionOn cmd_case block_case ite_case loop_case goto_case s)
+  | Stmt.goto label md => goto_case label md
+  termination_by s
 
 ---------------------------------------------------------------------
 
@@ -48,29 +79,22 @@ mutual
 @[simp]
 def Stmt.sizeOf (s : Imperative.Stmt P C) : Nat :=
   match s with
-  | .cmd c => 1 + sizeOf c
-  | .block _ ⟨ bss ⟩ _ => 1 + Stmts.sizeOf bss
-  | .ite c ⟨ tss ⟩ ⟨ ess ⟩ _ => 3 + sizeOf c + Stmts.sizeOf tss + Stmts.sizeOf ess
-  | .loop g _ _ ⟨ bss ⟩ _ => 3 + sizeOf g + Stmts.sizeOf bss
+  | .cmd c => 1 + SizeOf.sizeOf c
+  | .block _ bss _ => 1 + Block.sizeOf bss
+  | .ite c tss ess _ => 3 + sizeOf c + Block.sizeOf tss + Block.sizeOf ess
+  | .loop g _ _ bss _ => 3 + sizeOf g + Block.sizeOf bss
   | .goto _ _ => 1
 
 @[simp]
-def Stmts.sizeOf (ss : Imperative.Stmts P C) : Nat :=
+def Block.sizeOf (ss : Imperative.Block P C) : Nat :=
   match ss with
   | [] => 1
-  | s :: srest => 1 + Stmt.sizeOf s + Stmts.sizeOf srest
-
-@[simp]
-def Block.sizeOf : Imperative.Block P C →  Nat
-  | ⟨ bss ⟩ => 1 + Stmts.sizeOf bss
+  | s :: srest => 1 + Stmt.sizeOf s + Block.sizeOf srest
 
 end
 
 instance (P : PureExpr) : SizeOf (Imperative.Stmt P C) where
   sizeOf := Stmt.sizeOf
-
-instance (P : PureExpr) : SizeOf (Imperative.Stmts P C) where
-  sizeOf := Stmts.sizeOf
 
 instance (P : PureExpr) : SizeOf (Imperative.Block P C) where
   sizeOf := Block.sizeOf
@@ -88,19 +112,19 @@ mutual
 /-- Does statement `s` contain any block labeled `label`? -/
 def Stmt.hasLabelInside (label : String) (s : Stmt P C) : Bool :=
   match s with
-  |  .block label' ⟨ bss ⟩ _ => label = label' || Stmts.hasLabelInside label bss
-  |  .ite _ ⟨ tss ⟩ ⟨ ess ⟩  _ => Stmts.hasLabelInside label tss || Stmts.hasLabelInside label ess
+  |  .block label' bss _ => label = label' || Block.hasLabelInside label bss
+  |  .ite _ tss ess _ => Block.hasLabelInside label tss || Block.hasLabelInside label ess
   |  _ => false
   termination_by (Stmt.sizeOf s)
 
 /--
 Do statements `ss` contain any block labeled `label`?
 -/
-def Stmts.hasLabelInside (label : String) (ss : List (Stmt P C)) : Bool :=
+def Block.hasLabelInside (label : String) (ss : List (Stmt P C)) : Bool :=
   match ss with
   | [] => false
-  | s :: ss => Stmt.hasLabelInside label s || Stmts.hasLabelInside label ss
-  termination_by (Stmts.sizeOf ss)
+  | s :: ss => Stmt.hasLabelInside label s || Block.hasLabelInside label ss
+  termination_by (Block.sizeOf ss)
 end
 
 ---------------------------------------------------------------------
@@ -112,17 +136,17 @@ mutual
 def Stmt.getVars [HasVarsPure P P.Expr] [HasVarsPure P C] (s : Stmt P C) : List P.Ident :=
   match s with
   | .cmd cmd => HasVarsPure.getVars cmd
-  | .block _ ⟨ bss ⟩ _ => Stmts.getVars bss
-  | .ite _ ⟨ tbss ⟩ ⟨ ebss ⟩ _ => Stmts.getVars tbss ++ Stmts.getVars ebss
-  | .loop _ _ _ ⟨ bss ⟩ _ => Stmts.getVars bss
+  | .block _ bss _ => Block.getVars bss
+  | .ite _ tbss ebss _ => Block.getVars tbss ++ Block.getVars ebss
+  | .loop _ _ _ bss _ => Block.getVars bss
   | .goto _ _  => []
   termination_by (Stmt.sizeOf s)
 
-def Stmts.getVars [HasVarsPure P P.Expr] [HasVarsPure P C] (ss : Stmts P C) : List P.Ident :=
+def Block.getVars [HasVarsPure P P.Expr] [HasVarsPure P C] (ss : Block P C) : List P.Ident :=
   match ss with
   | [] => []
-  | s :: srest => Stmt.getVars s ++ Stmts.getVars srest
-  termination_by (Stmts.sizeOf ss)
+  | s :: srest => Stmt.getVars s ++ Block.getVars srest
+  termination_by (Block.sizeOf ss)
 end
 
 instance (P : PureExpr) [HasVarsPure P P.Expr] [HasVarsPure P C]
@@ -130,24 +154,24 @@ instance (P : PureExpr) [HasVarsPure P P.Expr] [HasVarsPure P C]
   getVars := Stmt.getVars
 
 instance (P : PureExpr) [HasVarsPure P P.Expr] [HasVarsPure P C]
-  : HasVarsPure P (Stmts P C) where
-  getVars := Stmts.getVars
+  : HasVarsPure P (Block P C) where
+  getVars := Block.getVars
 
 mutual
 /-- Get all variables defined by the statement `s`. -/
 def Stmt.definedVars [HasVarsImp P C] (s : Stmt P C) : List P.Ident :=
   match s with
   | .cmd cmd => HasVarsImp.definedVars cmd
-  | .block _ ⟨ bss ⟩  _ => Stmts.definedVars bss
-  | .ite _ ⟨ tbss ⟩ ⟨ ebss ⟩ _ => Stmts.definedVars tbss ++ Stmts.definedVars ebss
+  | .block _ bss _ => Block.definedVars bss
+  | .ite _ tbss ebss _ => Block.definedVars tbss ++ Block.definedVars ebss
   | _ => []
   termination_by (Stmt.sizeOf s)
 
-def Stmts.definedVars [HasVarsImp P C] (ss : Stmts P C) : List P.Ident :=
+def Block.definedVars [HasVarsImp P C] (ss : Block P C) : List P.Ident :=
   match ss with
   | [] => []
-  | s :: srest => Stmt.definedVars s ++ Stmts.definedVars srest
-  termination_by (Stmts.sizeOf ss)
+  | s :: srest => Stmt.definedVars s ++ Block.definedVars srest
+  termination_by (Block.sizeOf ss)
 end
 
 mutual
@@ -156,16 +180,16 @@ def Stmt.modifiedVars [HasVarsImp P C] (s : Stmt P C) : List P.Ident :=
   match s with
   | .cmd cmd => HasVarsImp.modifiedVars cmd
   | .goto _ _ => []
-  | .block _ ⟨ bss ⟩ _ => Stmts.modifiedVars bss
-  | .ite _ ⟨ tbss ⟩ ⟨ ebss ⟩ _ => Stmts.modifiedVars tbss ++ Stmts.modifiedVars ebss
-  | .loop _ _ _ ⟨ bss ⟩ _ => Stmts.modifiedVars bss
+  | .block _ bss _ => Block.modifiedVars bss
+  | .ite _ tbss ebss _ => Block.modifiedVars tbss ++ Block.modifiedVars ebss
+  | .loop _ _ _ bss _ => Block.modifiedVars bss
   termination_by (Stmt.sizeOf s)
 
-def Stmts.modifiedVars [HasVarsImp P C] (ss : Stmts P C) : List P.Ident :=
+def Block.modifiedVars [HasVarsImp P C] (ss : Block P C) : List P.Ident :=
   match ss with
   | [] => []
-  | s :: srest => Stmt.modifiedVars s ++ Stmts.modifiedVars srest
-  termination_by (Stmts.sizeOf ss)
+  | s :: srest => Stmt.modifiedVars s ++ Block.modifiedVars srest
+  termination_by (Block.sizeOf ss)
 end
 
 mutual
@@ -175,17 +199,17 @@ mutual
 @[simp]
 def Stmt.touchedVars [HasVarsImp P C] (s : Stmt P C) : List P.Ident :=
   match s with
-  | .block _ ⟨ bss ⟩ _ => Stmts.touchedVars bss
-  | .ite _ ⟨ tbss ⟩ ⟨ ebss ⟩ _ => Stmts.touchedVars tbss ++ Stmts.touchedVars ebss
+  | .block _ bss _ => Block.touchedVars bss
+  | .ite _ tbss ebss _ => Block.touchedVars tbss ++ Block.touchedVars ebss
   | _ => Stmt.definedVars s ++ Stmt.modifiedVars s
   termination_by (Stmt.sizeOf s)
 
 @[simp]
-def Stmts.touchedVars [HasVarsImp P C] (ss : Stmts P C) : List P.Ident :=
+def Block.touchedVars [HasVarsImp P C] (ss : Block P C) : List P.Ident :=
   match ss with
   | [] => []
-  | s :: srest => Stmt.touchedVars s ++ Stmts.touchedVars srest
-  termination_by (Stmts.sizeOf ss)
+  | s :: srest => Stmt.touchedVars s ++ Block.touchedVars srest
+  termination_by (Block.sizeOf ss)
 end
 
 instance (P : PureExpr) [HasVarsImp P C] : HasVarsImp P (Stmt P C) where
@@ -194,11 +218,11 @@ instance (P : PureExpr) [HasVarsImp P C] : HasVarsImp P (Stmt P C) where
   -- order matters for Havoc, so needs to override the default
   touchedVars := Stmt.touchedVars
 
-instance (P : PureExpr) [HasVarsImp P C] : HasVarsImp P (Stmts P C) where
-  definedVars := Stmts.definedVars
-  modifiedVars := Stmts.modifiedVars
+instance (P : PureExpr) [HasVarsImp P C] : HasVarsImp P (Block P C) where
+  definedVars := Block.definedVars
+  modifiedVars := Block.modifiedVars
   -- order matters for Havoc, so needs to override the default
-  touchedVars := Stmts.touchedVars
+  touchedVars := Block.touchedVars
 
 ---------------------------------------------------------------------
 
@@ -211,22 +235,22 @@ partial def formatStmt (P : PureExpr) (s : Stmt P C)
   [ToFormat P.Ident] [ToFormat P.Expr] [ToFormat P.Ty] [ToFormat C] : Format :=
   match s with
   | .cmd cmd => format cmd
-  | .block label bl md => f!"{md}{label} : " ++ Format.bracket "{" f!"{formatStmts P bl.ss}" "}"
+  | .block label bl md => f!"{md}{label} : " ++ Format.bracket "{" f!"{formatBlock P bl}" "}"
   | .ite cond th el md => f!"{md}if {cond} then " ++
-                        Format.bracket "{" f!"{formatStmts P th.ss}" "}" ++
+                        Format.bracket "{" f!"{formatBlock P th}" "}" ++
                         f!"{Format.line}else" ++
-                        Format.bracket "{" f!"{formatStmts P el.ss}" "}"
+                        Format.bracket "{" f!"{formatBlock P el}" "}"
   | .loop guard measure invariant body md => f!"{md}while ({guard}) ({measure}) ({invariant}) " ++
-                        Format.bracket "{" f!"{formatStmts P body.ss}" "}"
+                        Format.bracket "{" f!"{formatBlock P body}" "}"
   | .goto label md => f!"{md}goto {label}"
 
-partial def formatStmts (P : PureExpr) (ss : List (Stmt P C))
+partial def formatBlock (P : PureExpr) (ss : List (Stmt P C))
   [ToFormat P.Ident] [ToFormat P.Expr] [ToFormat P.Ty] [ToFormat C] : Format :=
     match ss with
     | [] => f!""
     | s :: rest => formatStmt P s ++
                    if rest.isEmpty then f!""
-                   else f!"\n{formatStmts P rest}"
+                   else f!"\n{formatBlock P rest}"
 end
 
 instance [ToFormat P.Ident] [ToFormat P.Expr] [ToFormat P.Ty]
@@ -239,7 +263,7 @@ instance [ToFormat P.Ident] [ToFormat P.Expr] [ToFormat P.Ty] [ToFormat C]
 
 instance [ToFormat P.Ident] [ToFormat P.Expr] [ToFormat P.Ty] [ToFormat C]
         : ToFormat (List (Stmt P C)) where
-  format ss := formatStmts P ss
+  format ss := formatBlock P ss
 
 ---------------------------------------------------------------------
 
